Typechecking for teleportation example

examples/HOASTeleportation.v
@@ -15,7 +15,7 @@ Definition teleport (Alice Bob : Actor.t) (q : Var.t) : Qoreo Var.t :=
       do (q,a) ← Alice [-- Unitary CNOT (Pair q a) -] ;;
       do q     ← Alice [- Unitary H q -] ;;
       do x ← Alice [- Meas q -];;
-      do z ← Alice [- Meas q -];;
+      do z ← Alice [- Meas a -];;
 
       (* Alice sends x and z to Bob. *)
       do x ← send Alice x Bob ;;
@@ -25,6 +25,231 @@ Definition teleport (Alice Bob : Actor.t) (q : Var.t) : Qoreo Var.t :=
       do b ← Bob [- If z (Unitary Z b) b -];;
       do b ← Bob [- If x (Unitary X b) b -];;
       ret b.
+
+About Choreography.WellTyped.
+Import Actor.Map.
+Require Import Lia.
+
+Lemma remove_empty : forall A x T,
+  ChorEnv.Equal (ChorEnv.remove A x (empty (Var.Map.t T))) (empty _).
+Admitted.
+Hint Rewrite remove_empty : var_db.
+
+Definition singleton {T} x (tau : T) := Var.Map.add x tau (Var.Map.empty T).
+Lemma wtqvar : forall x (τ : typ),
+  Expr.WellTyped (Var.Map.empty _) (Var.Map.add x τ (Var.Map.empty _)) (Var.Map.empty _) (Expr.Var x) τ.
+Proof.
+  intros. econstructor; eauto; Var.simplify.
+Qed.
+Lemma wtbit : forall Γ b,
+  Expr.WellTyped Γ (Var.Map.empty _) (Var.Map.empty _) (Bit b) BIT.
+Proof. intros. econstructor; eauto; Var.simplify. Qed.
+
+Lemma wtqref : forall Γ q (idx : nat),
+  Expr.WellTyped Γ (Var.Map.empty _) (Var.Map.add q idx (Var.Map.empty _)) (QRef q) QUBIT.
+Proof. intros. econstructor; eauto; Var.simplify. Qed.
+
+
+Ltac solve_wt :=
+  match goal with
+  | [ |- Expr.WellTyped _ _ _ (Expr.Var ?q) _ ] => apply wtqvar
+  | [ |- Expr.WellTyped _ _ _ (Bit _) _] => apply wtbit
+  | [ |- Expr.WellTyped _ _ _ (QRef _) _] => apply wtqref
+  | [ |- Expr.WellTyped _ _ _ _ _] => econstructor; auto; try reflexivity
+  | [ |- Choreography.WellTyped _ _ _ _] => econstructor; auto; try reflexivity
+
+  | [ |- Var.Map.Partition _ _ _ ] => Var.Map.Tactics.reflect_partition
+  | [ |- _ /\ _ ] => split; auto
+  | [ |- ~ (_ \/ _)] => intros [? | ?]; subst; try contradiction
+  end.
+
+
+Lemma ce_add_empty : forall T (m : ChorEnv.t T) A,
+  ChorEnv.Equal
+    (Actor.Map.add A (Var.Map.empty _) m)
+    (Actor.Map.remove A m).
+Proof.
+  intros T m A.
+  intros B. ChorEnv.simplify.
+Qed.
+Hint Rewrite ce_add_empty : var_db.
+Hint Rewrite @Choreography.addadd2 : var_db.
+
+Lemma ce_remove_empty : forall A,
+    ChorEnv.Equal (Actor.Map.remove A (Actor.Map.empty (Var.Map.t nat))) (Actor.Map.empty _).
+Proof. intros. ChorEnv.simplify. Qed.
+Hint Rewrite ce_remove_empty : var_db.
+
+(* TODO: improve tactics for typechecking! *)
+Lemma WellTyped_teleport : forall Alice Bob q C,
+  Alice <> Bob ->
+  q = 10 (* ensure q is fresh in teleport *) ->
+  WellTyped (empty _) (ChorEnv.add Bob q QUBIT (empty _)) (empty _) C ->
+  WellTyped (empty _) (ChorEnv.add Alice q QUBIT (empty _)) (empty _)
+    (mk (teleport Alice Bob q) ++ C)%list.
+Proof.
+  intros Alice Bob q C Hneq Hfresh HWT.
+  remember (mk (teleport Alice Bob q)) as C0 eqn:HC0.
+  cbv in HC0. subst.
+
+  solve_wt; ChorEnv.simplify.
+
+  econstructor.
+  { repeat (solve_wt; ChorEnv.simplify). }
+  2:{
+    ChorEnv.simplify.
+    Var.Map.Tactics.reflect_partition.
+    { apply Var.Map.Proofs.disjoint_empty_2. }
+    { Var.solve. }
+  }
+  2:{
+    Var.Map.Tactics.reflect_partition.
+    apply Var.Map.Proofs.disjoint_empty_2.
+    Var.solve.
+  }
+  2:{ Var.simplify. }
+  2:{ Var.simplify. }
+
+
+  ChorEnv.simplify.
+  econstructor.
+  { repeat (solve_wt; ChorEnv.simplify). }
+  2:{
+    ChorEnv.simplify.
+    instantiate (1 := (Var.Map.add 3 QUBIT (Var.Map.empty typ))).
+    repeat (solve_wt; ChorEnv.simplify).
+  }
+  2:{
+    ChorEnv.simplify.
+    auto with var_db.
+  }
+  2:{ Var.simplify. }
+
+
+  ChorEnv.simplify.
+  econstructor.
+  { repeat solve_wt. }
+  2:{
+    ChorEnv.simplify.
+    instantiate (1 := (Var.Map.add 3 QUBIT (Var.Map.empty typ))).
+    repeat (solve_wt; ChorEnv.simplify).
+  }
+  2:{ ChorEnv.simplify. auto with var_db. }
+  2:{ Var.simplify. }
+
+  ChorEnv.simplify.
+  match goal with
+  | [ |- WellTyped _ ?D _ _ ] =>
+    assert (Heq : ChorEnv.Equal D (ChorEnv.add Alice 5 (BANG BIT) (ChorEnv.add Alice 3 QUBIT (ChorEnv.add Bob 1 QUBIT (empty (Var.Map.t _))))))
+  end.
+  { intros D. ChorEnv.simplify. }
+  rewrite Heq. clear Heq.
+
+  econstructor.
+  { repeat solve_wt. }
+  2:{
+    ChorEnv.simplify.
+    instantiate (1 := (Var.Map.add 5 (BANG BIT) (Var.Map.empty typ))).
+    repeat (solve_wt; ChorEnv.simplify).
+    Search (Var.Map.add _ _ (Var.Map.add _ _ _)).
+    rewrite Var.Map.Proofs.add_neq_sym; auto.
+    reflexivity.
+  }
+  2:{ ChorEnv.simplify. auto with var_db. }
+  2:{ Var.simplify. }
+
+  ChorEnv.simplify. unfold ChorEnv.add. ChorEnv.simplify.
+
+  econstructor; auto.
+  { repeat solve_wt. }
+  2:{
+    ChorEnv.simplify.
+    instantiate (1 := (Var.Map.add 6 (BANG BIT) (Var.Map.empty typ))).
+    repeat (solve_wt; ChorEnv.simplify).
+    Var.solve.
+  }
+  2:{ ChorEnv.simplify. auto with var_db. }
+
+  ChorEnv.simplify.
+  econstructor; auto.
+  { ChorEnv.simplify.
+    solve_wt.
+  }
+  2:{
+    ChorEnv.simplify.
+    instantiate (1 := (Var.Map.empty typ)).
+    repeat (solve_wt; ChorEnv.simplify).
+  }
+  2:{ ChorEnv.simplify. auto with var_db. }
+
+
+  ChorEnv.simplify.
+  match goal with
+  | [ |- WellTyped _ ?D _ _ ] =>
+    assert (Heq : ChorEnv.Equal D (ChorEnv.add Bob 1 QUBIT (empty _)))
+  end.
+  { intros B. ChorEnv.simplify. }
+  rewrite Heq. clear Heq.
+  econstructor; auto.
+  {
+    ChorEnv.simplify.
+    solve_wt.
+    { apply Expr.WTCVar; Var.simplify; eauto with var_db. }
+    { apply Expr.weakening. solve_wt. solve_wt; eauto with var_db.
+      Var.simplify. repeat solve_wt; auto with var_db. lia. lia.
+    } 
+    { apply Expr.weakening. solve_wt.
+      Var.simplify. repeat solve_wt; auto with var_db. lia. lia.
+    }
+    { auto with var_db. }
+    { auto with var_db. }
+  }
+  2:{
+    ChorEnv.simplify.
+    auto with var_db.
+  }
+  2:{ ChorEnv.simplify. auto with var_db. }
+  2:{ Var.simplify. }
+
+  ChorEnv.simplify. simpl.
+  econstructor; auto.
+  {
+    ChorEnv.simplify.
+    solve_wt.
+    { apply Expr.WTCVar; Var.simplify; eauto with var_db. }
+    { apply Expr.weakening. solve_wt. simpl. solve_wt; eauto with var_db.
+      Var.simplify. repeat solve_wt; auto with var_db. lia.
+    } 
+    { apply Expr.weakening. solve_wt.
+      Var.simplify. repeat solve_wt; auto with var_db. lia.
+    }
+    { auto with var_db. }
+    { auto with var_db. }
+  }
+  2:{
+    ChorEnv.simplify.
+    auto with var_db.
+  }
+  2:{ ChorEnv.simplify. auto with var_db. }
+  2:{ Var.simplify. }
+
+  ChorEnv.simplify.
+  match goal with
+  | [ |- WellTyped ?G ?D _ _ ] =>
+    assert (Heq : ChorEnv.Equal G (ChorEnv.add Bob 8 BIT (ChorEnv.add Bob 7 BIT (Actor.Map.empty _))));
+    [ | assert (Heq' : ChorEnv.Equal D (ChorEnv.add Bob 10 QUBIT (empty _)))]
+  end.
+  { intros B. ChorEnv.simplify. }
+  { intros B. ChorEnv.simplify. }
+  rewrite Heq, Heq'. clear Heq Heq'.
+
+  eapply Choreography.weakening_gen with (G := empty (Var.Map.t typ)) (G0 := ChorEnv.add Bob 8 BIT (ChorEnv.add Bob 7 BIT (empty _))).
+  2:{
+    intros B. split. ChorEnv.simplify; auto with var_db.
+    ChorEnv.simplify. repeat solve_wt; auto with var_db; lia.
+  }
+  auto.
+Qed.
 
 Definition choreo : Choreography.t :=
   mk (
